src/traits.rs
@@ -1,0 +1,79 @@
+use syntax;
+use syntax::ast;
+use rustc::middle::infer;
+use rustc::middle::subst;
+use rustc::middle::traits;
+use rustc::middle::ty::*;
+use rustc::middle::def_id::DefId;
+//use rustc_trans::trans::monomorphize;
+
+// copied from trans::meth
+fn combine_impl_and_methods_tps<'tcx>(tcx: &ctxt<'tcx>,
+                                      node_substs: subst::Substs<'tcx>,
+                                      rcvr_substs: subst::Substs<'tcx>)
+                                      -> subst::Substs<'tcx>
+{
+    // Break apart the type parameters from the node and type
+    // parameters from the receiver.
+    let node_method = node_substs.types.split().fns;
+    let subst::SeparateVecsPerParamSpace {
+        types: rcvr_type,
+        selfs: rcvr_self,
+        fns: rcvr_method
+    } = rcvr_substs.types.clone().split();
+    assert!(rcvr_method.is_empty());
+    subst::Substs {
+        regions: subst::ErasedRegions,
+        types: subst::VecPerParamSpace::new(rcvr_type, rcvr_self, node_method)
+    }
+}
+
+// copied from trans::common
+fn fulfill_obligation<'tcx>(tcx: &ctxt<'tcx>, trait_ref: PolyTraitRef<'tcx>)
+    -> traits::Vtable<'tcx, ()>
+{
+    let span = syntax::codemap::DUMMY_SP;
+    let infcx = infer::normalizing_infer_ctxt(tcx, &tcx.tables);
+    let mut selcx = traits::SelectionContext::new(&infcx);
+    let obligation =
+        traits::Obligation::new(traits::ObligationCause::misc(span, ast::DUMMY_NODE_ID),
+        trait_ref.to_poly_trait_predicate());
+    let selection = selcx.select(&obligation).unwrap().unwrap();
+    let mut fulfill_cx = infcx.fulfillment_cx.borrow_mut();
+    let vtable = selection.map(|predicate| {
+        fulfill_cx.register_predicate_obligation(&infcx, predicate);
+    });
+    infer::drain_fulfillment_cx_or_panic(
+        span, &infcx, &mut fulfill_cx, &vtable
+    )
+}
+
+pub fn lookup_trait_item_impl<'tcx>(tcx: &ctxt<'tcx>, item_did: DefId, substs: &subst::Substs<'tcx>) -> Option<DefId> {
+    tcx.trait_of_item(item_did).map(|trait_did| {
+        // from trans::meth::trans_method_callee
+        let trait_substs = substs.clone().method_to_trait();
+        let trait_substs = tcx.mk_substs(trait_substs);
+        let trait_ref = TraitRef::new(trait_did, trait_substs);
+        let trait_ref = Binder(trait_ref);
+        match fulfill_obligation(tcx, trait_ref) {
+            traits::Vtable::VtableImpl(data) => {
+                // from trans::meth::trans_monomorphized_callee
+                let impl_did = data.impl_def_id;
+                let mname = match tcx.impl_or_trait_item(item_did) {
+                    MethodTraitItem(method) => method.name,
+                    _ => unreachable!(),
+                };
+                //println!("substs: {:?}, trait_substs: {:?}, vtable: {:?}", substs, trait_substs, data.substs);
+                let callee_substs = combine_impl_and_methods_tps(tcx, substs.clone(), data.substs);
+                //println!("callee_substs: {:?}", callee_substs);
+                //println!("impl_did: {:?}", tcx.def_path(impl_did));
+
+                let mth = tcx.get_impl_method(impl_did, callee_substs, mname);
+                //println!("lookup: {:?}", mth);
+                mth.method.def_id
+            },
+            _ => panic!("unimplementd: {:?}", trait_ref),
+        }
+    })
+}
+
