Prove.thy
@@ -2,37 +2,17 @@ theory Prove
 imports Export Binomial
 begin
 
-(*
-lemma fac_16:
-  assumes "s 3 = core_option_Option_Some (Any_3 (core_ops_Range 2 n))"
-  shows "fac_16 (\<lambda>s. case s (Suc 0) of Some (Any_1 xa) \<Rightarrow> xa) s = fact n"
-proof-
-  have "fac_16_dom (\<lambda>a. fac_16 (\<lambda>s. case s (Suc 0) of Some (Any_1 xa) \<Rightarrow> xa) a = fact n, s)"
-  thm fac_16.domintros
-  apply (rule fac_16.domintros)
-  apply (auto split:option.splits)
-
-  
-  apply (rule fac_16.pinduct)
-*)
-
-lemma "(s(1:=1,2:=2,3:=3)) 2 = 2" by simp
-find_theorems "_(?x:=_,?y := _ )"
-lemma "(case if b then Some x else None of Some x \<Rightarrow> P x | None \<Rightarrow> Q) = P x" by simp
 lemma fac: "fac (n::u32) = fact n"
 proof-
-  let ?s = "
-     (Map.empty(0 := core_option_Option_Some (Any_0 n), Suc 0 := core_option_Option_Some (Any_1 (Suc 0)), 8 := core_option_Option_Some (Any_8 core_iter_I_IntoIterator_into_iter),
-                10 := core_option_Option_Some (Any_10 n), 9 := core_option_Option_Some (Any_9 (core_ops_Range 2 n)), 7 := core_option_Option_Some (Any_7 (core_ops_Range 2 n)),
-                3 := core_option_Option_Some (Any_3 (core_ops_Range 2 n))))"
   show ?thesis
   unfolding fac_def
   apply auto
-  apply (rule loop_rule[where P="\<lambda>s. \<exists>k. s 9 = Some (Any_9 (core_ops_Range k n))"])
-  apply (auto simp: fac_16_def)[1]
-  apply (simp add: fac_16_def split:prod.splits core_ops_Range.splits)
-  apply (cases "2<n")
+  apply (rule loop_rule[where P="\<lambda>s. case s of (res,core_ops_Range (Suc l) r) \<Rightarrow> res = fact l \<and> (n = 0 \<and> l = 1 \<or> l < r) \<and> r = n+1 | _ \<Rightarrow> False"])
+  unfolding fac_16_def
   apply auto[1]
+  apply (auto simp add: le_less_Suc_eq split:prod.splits core_ops_Range.splits split_if_asm option.splits nat.splits)[2]
+  apply (rule wf_measure[of "\<lambda>s. case s of (_,core_ops_Range l r) \<Rightarrow> r-l"])
+  by (auto simp add: le_less_Suc_eq split:prod.splits core_ops_Range.splits split_if_asm option.splits nat.splits)
 qed
 
 end
